added documentation to heap allocator proofs

Proofs/Memory.thy
@@ -4,9 +4,13 @@ theory Memory
     "../lib/ExtraLemmas"
     "./Memory_Nodes"
     "./Memory_ExtraLemmas"
-    "~/Isabelle2016-1/src/HOL/Library/LaTeXsugar"
-    
+    "~/Isabelle2016-1/src/HOL/Library/LaTeXsugar"    
 begin
+text \<open>This theory file proves correctness of the heap allocator's alloc() function.
+      The required supporting definitions and lemmas come first, they are followed by a lemma
+      that states alloc() preserves a set of invariants, and at the end the
+      lemma that states that alloc() is correct given the invariants as a precondition
+      is proved\<close> 
   
 context sable_isa
 begin
@@ -27,13 +31,10 @@ lemma[dest, intro]: "mem_node_C_guard p \<Longrightarrow> c_guard p"
   unfolding mem_node_C_guard_def c_guard_def ptr_aligned_def is_aligned_def
   by (auto simp add: align_of_def, unat_arith)
     
-lemma contrapos: "(P \<longrightarrow> Q) = (\<not>Q \<longrightarrow> \<not>P)"
-  by blast
-    
 definition
   liftC :: "('c \<Rightarrow> 'a) \<Rightarrow> ('c \<Rightarrow> bool) \<Rightarrow> ('a \<Rightarrow> bool)"
-  where
-    "liftC st P \<equiv> \<lambda>s. \<forall>g. s = st g \<longrightarrow> P g"
+where
+  "liftC st P \<equiv> \<lambda>s. \<forall>g. s = st g \<longrightarrow> P g"
     
 lemma hoare_liftC_wp[wp]:
   "\<lbrace>P\<rbrace> m \<lbrace>\<lambda>r s. \<forall>t. st s = t \<longrightarrow> Q r t\<rbrace> \<Longrightarrow> \<lbrace>liftC st P\<rbrace> exec_concrete st m \<lbrace>Q\<rbrace>"
@@ -64,7 +65,10 @@ definition nodeFree :: "globals \<Rightarrow> mem_node_C ptr \<Rightarrow> bool"
     (let size = node_size_masked s node in
     \<forall>p \<in> {ptr_val (node +\<^sub>p 1)..+unat size * SZ_mem_node}.
       snd (hrs_htd (t_hrs_' s) p) = Map.empty)"
-    
+
+text \<open>the nodeValid predicate defines the constraints on each node that alloc()
+      must preserve. It is not defined in the most straightforward fashion possible, but it is
+      valid nonetheless\<close>    
 definition nodeValid :: "globals \<Rightarrow> mem_node_C ptr \<Rightarrow> bool"
   where "nodeValid s node = 
   (let occupied = node_size s node && scast OCC_FLG in
@@ -122,13 +126,17 @@ lemma nodeValid_node_size_upper_bound:
   apply (subgoal_tac "ptr_val node \<noteq> 0") 
   using word_neq_0_conv apply blast
   by (metis ptr.exhaust ptr_val.ptr_val_def)
-    
-function nodesValid :: "globals \<Rightarrow> mem_node_C ptr \<Rightarrow> bool" where
-  "\<not> (nodeValid s heap) \<Longrightarrow> nodesValid s heap = False"
+
+text \<open>This is essentially the definition of the heap invariants that alloc() must preserve.
+      It requires all the nodes in the linked list to be valid\<close>
+function 
+  nodesValid :: "globals \<Rightarrow> mem_node_C ptr \<Rightarrow> bool" 
+where
+ "\<not> (nodeValid s heap) \<Longrightarrow> nodesValid s heap = False"
 |"nodeValid s heap \<and> node_next s heap = NULL \<Longrightarrow> nodesValid s heap = True"
 |"nodeValid s heap \<and> node_next s heap \<noteq> NULL \<Longrightarrow> nodesValid s heap =
-      nodesValid s (node_next s heap)"
-        apply auto by blast 
+      nodesValid s (node_next s heap)" 
+     apply auto by blast
 termination
   apply (relation "measure (\<lambda> (s,heap). 2 ^ 32 - unat_ptr heap)")
    apply auto
@@ -136,16 +144,15 @@ termination
   apply (clarsimp simp:ptr_less_simp ptr_le_simp)
   by unat_arith auto
     
-lemma nodesValid_def' :"nodesValid s heap =
+text \<open>a simplified definition of nodesValid, equivalent to the real definition\<close>   
+lemma nodesValid_def': "nodesValid s heap =
   (let next = (node_next s heap) in 
     nodeValid s heap \<and> (next \<noteq> NULL \<longrightarrow> nodesValid s next))"
   unfolding Let_def
-  using nodesValid.simps
-  by blast
+  using nodesValid.simps by blast
   
 definition heap_invs :: "globals \<Rightarrow> unit ptr \<Rightarrow> bool"
-  where
-    "heap_invs s heap \<equiv> nodesValid s (ptr_coerce heap)"
+where "heap_invs s heap \<equiv> nodesValid s (ptr_coerce heap)"
     
 lemma nodesValid_nodeValid: "nodesValid s n \<Longrightarrow> nodeValid s n"
   apply(subst (asm) nodesValid_def') unfolding Let_def by auto
@@ -161,7 +168,11 @@ lemma heap_invs_not_null :"heap_invs s heap \<Longrightarrow> heap \<noteq> NULL
 lemma nodesValid_not_next_null:
   "nodesValid s node \<Longrightarrow> \<not> nodesValid s (node_next s node) \<Longrightarrow> (node_next s node) = NULL"
   using nodesValid.elims by auto 
-    
+
+text \<open>reachable is a predicate returning true when node `to` is reachable from node `node` in the
+      linked list. Its definition is split into multiple cases to make proving totality of the
+      function possible, in addition the next node of each node must be at a higher address than
+      the node for totality to be provable \<close>    
 function  reachable :: "globals \<Rightarrow> mem_node_C ptr \<Rightarrow> mem_node_C ptr \<Rightarrow> bool"
   where "reachable s NULL to = (to = NULL)"
   | "node \<noteq> NULL \<and> node = to \<Longrightarrow> reachable s node to = True"
@@ -211,7 +222,6 @@ lemma reachable_trans[rule_format]:
   apply (rule reachable.simps(4)[THEN iffD2])
    apply auto
    apply (drule_tac node="node_next s (node_next s to)" in reachable_helper2)
-    apply simp
   by (auto simp: ptr_le_simp ptr_less_simp)  
     
 lemma reachable_trans2[rule_format]:
@@ -219,7 +229,8 @@ lemma reachable_trans2[rule_format]:
    reachable s node (node_next s to)"
   apply (rule_tac ?a0.0=s and ?a1.0=node and ?a2.0=to in  reachable.induct)
   by auto
-    
+
+text \<open> the memory outside an updated linked list node remains untouched \<close>
 lemma updated_node_hrs_the_same_elsewhere:
   assumes x_val:"x \<notin> ptr_span p"
   shows"hrs_the_same_at s (update_node s p new_node) x"
@@ -263,7 +274,12 @@ proof-
     using `hrs_the_same_at s ?halfway_s x`
     by simp
 qed
-    
+
+text \<open>This function returns all the nodes in path from node `node` to node `to` (excluding `to`).
+      Each node in the path must be at a higher address than its previous node. In addition to 
+      being a reflection of the heap allocator implementation, this requirement makes the path 
+      function a total function (a function with a defined value for every combination of parameters).
+      Totality is required in Isabelle for all functions \<close>
 function path :: "globals \<Rightarrow> mem_node_C ptr \<Rightarrow> mem_node_C ptr \<Rightarrow> mem_node_C ptr list"
   where "node = NULL \<or> node \<ge> node_next s node \<or> node_next s node > to \<Longrightarrow>
           path s node to = []"
@@ -274,6 +290,9 @@ function path :: "globals \<Rightarrow> mem_node_C ptr \<Rightarrow> mem_node_C 
      apply auto 
   by (metis  dual_order.strict_iff_order le_cases)
 termination
+  text \<open> introducing a function that is monotonically decreasing with each recursive call
+        is the way to prove wellfoundedness of the relation between recursive parameters,
+        which in turn proves totality \<close>
   apply (relation "measure (\<lambda> (s,node,to).2 ^ 32 + unat_ptr to - unat_ptr node)")
    apply (auto simp:ptr_less_simp ptr_le_simp)
   by unat_arith     
@@ -282,8 +301,8 @@ lemma path_not_empty_node_cond[rule_format]: "set (path s node to) \<noteq> {} \
         node \<noteq> NULL \<and>
         ptr_val node < ptr_val (node_next s node) \<and>
         ptr_val node < ptr_val to \<and> ptr_val (node_next s node) \<le> ptr_val to"
-  apply (simp add:ptr_less_simp[THEN sym] ptr_le_simp[THEN sym] )
-  apply (rule contrapos[THEN iffD2])
+  apply (simp add:ptr_less_simp[THEN sym] ptr_le_simp[THEN sym])
+  apply (subst contrapos)
   apply (clarsimp)
   apply (rule path.simps)
   by auto
@@ -321,6 +340,8 @@ lemma p_in_path_l_next[rule_format]:
   apply (rule_tac ?a0.0=s and ?a1.0=node and ?a2.0=to in path.induct)
   by auto
 
+text \<open>if a valid node is at the last possible place in the address space (2 ^ 32 - 8),
+      then it must have size 0\<close>
 lemma nodeValid_edge_of_addr_space:
   assumes "nodeValid s node"
   shows "(node +\<^sub>p 1) > node \<or> (node_size_masked s node) = 0"
@@ -345,7 +366,10 @@ proof -
       by unat_arith auto
   } thus ?thesis by fast
 qed
-  
+
+text \<open> if the footprint of a node, and the heap memory corresponding to the node 
+      in two states are the same, and the node is valid in one state, 
+      then it is valid in the other state as well \<close>  
 lemma hrs_the_same_imp_nodeValid:
   "\<forall> p \<in> ptr_span node. hrs_the_same_at s s' p \<Longrightarrow>
    \<forall> p \<in> array_span (node +\<^sub>p 1) (unat (node_size_masked s node)). hrs_the_same_at s s' p \<Longrightarrow>   
@@ -631,6 +655,8 @@ proof -
   thus ?thesis using assms by (simp add: mask_eq_0_eq_x)
 qed
 
+text \<open>If a node n is in the path of another node fst_node, and nodesValid holds
+      for fst_node, then n must be a valid node \<close>
 lemma node_in_path_nodesValid_imp_nodeValid_node[rule_format]:
   "n \<in> set (path s fst_node to) \<longrightarrow> 
    nodesValid s fst_node \<longrightarrow>
@@ -641,6 +667,8 @@ lemma node_in_path_nodesValid_imp_nodeValid_node[rule_format]:
   apply (frule nodesValid_not_next_null)
   by auto
 
+text \<open> if there is a node 'to' reachable from node 'node', then 'node' must be in its
+      path to 'to', in other words, its path is not empty\<close>
 lemma node_reachable_in_path[rule_format]:
   "reachable s node to \<longrightarrow> node \<noteq> to\<longrightarrow> to \<noteq> NULL \<longrightarrow> node \<in> set (path s node to )"
   apply(rule_tac ?a0.0=s and ?a1.0=node and ?a2.0=to in reachable.induct)
@@ -755,13 +783,15 @@ next
     using nodeValid_heaps_eq_imp_nodeValid by blast
   ultimately show "nodesValid s' heap" using nodesValid_trans_back by fast
 qed 
-  
+
+text \<open>if nodesValid holds for 'node', and all the nodes in the path from
+      'heap' to 'node' are valid, then nodesValid holds for 'heap'\<close>
 lemma path_nodeValid_reachable_imp_nodesValid[rule_format]:
   "nodeValid s heap \<longrightarrow>
-       (\<forall> p \<in> set (path s heap node). nodeValid s p) \<longrightarrow>
-       reachable s heap node \<longrightarrow>
-       nodesValid s node \<longrightarrow>
-       nodesValid s heap"
+   (\<forall> p \<in> set (path s heap node). nodeValid s p) \<longrightarrow>
+   reachable s heap node \<longrightarrow>
+   nodesValid s node \<longrightarrow>
+   nodesValid s heap"
   apply (rule_tac ?a0.0=s and ?a1.0=heap and ?a2.0=node in path.induct) 
    apply (unfold nodeValid_def)[1] unfolding Let_def
    apply clarify
@@ -836,13 +866,19 @@ qed
 lemma OCC_FLG_neg : "(scast (~~ MEM_NODE_OCCUPIED_FLAG) ::32 word) = ~~ scast MEM_NODE_OCCUPIED_FLAG"
   by (metis (no_types) mask_eq_0_eq_x l11 mask_sw32_eq_0_eq_x word_bw_comms(1) word_log_esimps(7) 
       word_log_esimps(9) word_not_not)    
-  
+
+text \<open>This lemma states that alloc() preserves the invariants. As the size of this proof
+      suggests, most of the verification effort of alloc() was spent proving this lemma. \<close>    
 lemma alloc'_invs:
   fixes size_bytes:: "32 word" and heap:: "unit ptr"
   assumes size_bytes_g0 : "size_bytes > 0"
   shows "\<lbrace>\<lambda>s. heap_invs s heap \<rbrace> (alloc' heap size_bytes) \<lbrace> \<lambda>r s. heap_invs s heap \<rbrace>"
   unfolding alloc'_def Let_def 
   apply (simp add: h_val_field_from_bytes)
+    
+  text \<open>We are introducing all the loop invariants in this command. By introducing the lemmas,
+        'wp' will process the loop, and keeps the invariants as preconditions after the loop is done.
+         \<close>
   apply (subst whileLoop_add_inv 
       [where I="\<lambda> (n,r) s. heap_invs s heap \<and> reachable s (ptr_coerce heap) n
                   \<and> (r=0 \<longrightarrow> (n = NULL \<or> ((size_bytes >> 3) + 1
@@ -856,8 +892,11 @@ lemma alloc'_invs:
      apply (simp add: size_bytes_g0)
      apply (rule return_wp) 
   unfolding heap_invs_def
-  using [[simp_trace=false]] using [[simp_trace_depth_limit=1000]]
     apply (auto)
+    
+  text \<open>Applying auto breaks the proof into multiple subgoals, all of which except two are
+        trivially discharged. We discharge the trivial ones here, and leave the two main 
+        subgoals for later.\<close>
                     apply(drule c_guard_NULL, drule nodesValid_reachable_imp_next_reachable, auto)+  
                  apply (drule one_mask_neg_MNOF_not_zero, solves simp)
                 apply(drule c_guard_NULL, drule nodesValid_reachable_imp_next_reachable, auto)+
@@ -874,6 +913,9 @@ lemma alloc'_invs:
     apply (drule nodesValid_not_null, simp)
     apply (frule mask_sw32_eq_0_eq_x, solves simp)
    apply (frule nodesValid_not_null, simp)
+    
+text \<open>This subgoal corresponds to the case where a free slot in the heap of exactly the 
+      right size has been found \<close>
 proof -
   fix a::"mem_node_C ptr"
   fix s::globals
@@ -1046,7 +1088,11 @@ proof -
       using `nodesValid ?new_s a` by simp
   }    
   ultimately show "nodesValid ?new_s ?heap_node" by fastforce
+     
 next 
+text \<open>This subgoal corresponds to the case where the found slot in the heap is bigger than
+      the requested size, and so a new free node must be created at the end of the allocated memory
+      for the extra free space.\<close>
   fix a::"mem_node_C ptr"
   fix s::globals
   let ?node_size_masked = "node_size s a && scast (~~ OCC_FLG)"
@@ -1675,6 +1721,11 @@ next
   thus "nodesValid ?new_s_real (ptr_coerce heap)" by auto
 qed  
 
+text \<open>a helper theorem for alloc'_hoare, it proves the main goals for alloc'_hoare after it 
+      has gone through wp. The main goals correspond to the two branches of alloc(), one where
+      a free portion of exactly the correct size has been found, another where a free portion
+      bigger than the required size has been found. For the purposes of alloc'_hoare, the
+      preconditions required for the two branches turn out to be the same \<close>
 lemma alloc'_hoare_helper:
   fixes size_bytes heap
   assumes n:"size_of TYPE('a) \<le> unat size_bytes"
@@ -1788,7 +1839,10 @@ proof -
     thus "c_null_guard (ptr_coerce (node +\<^sub>p 1):: 'a ptr)" unfolding c_null_guard_def by blast  
   qed
 qed
-  
+
+text \<open>This is the main theorem. It proves that given the heap_invs precondition, if the returned 
+      pointer is not NULL, it is of the correct size, it is properly aligned with respect to the type the memory 
+      is being allocated for, and it points to a previously free (untyped) portion of the heap\<close>  
 lemma alloc'_hoare:
   fixes size_bytes :: "32 word"
   assumes align: "align_of TYPE('a) dvd align_of TYPE(mem_node_C)"
@@ -1857,7 +1911,6 @@ proof -
     and "\<forall>g. lift_global_heap b = lift_global_heap g \<longrightarrow> heap_invs g"
   hence "heap_invs s" and "heap_invs b" by auto
   oops *)
-    
 end
   
 end
